Merge memory and state/trace relations
The existing proof structure looks like it will adapt fairly well to
the richer setting of memory sharing, but some proofs require more
information than is currently available from the simple memory relation
devised to keep track of that region of the states. By integrating this
memory relation in the standard state mergeability relation and
establishing the necessary connections, we can begin to repair some of
the results that will be necessary to restore the basic building blocks
of the recombination proof.

Intermediate/RecombinationRel.v
@@ -285,17 +285,16 @@ Section Mergeable.
 
   (* Sketch a simple state relation based on the memory-trace relation, for the
      sake of expediency. *)
-  Inductive mergeable_states (s s' s'' : CS.state) : Prop :=
-  | mergeable_states_intro : forall t t' t'',
-      mem_rel3 (CS.state_mem s, t) (CS.state_mem s', t') (CS.state_mem s'', t'') ->
-      mergeable_states s s' s''.
+  (* Inductive mergeable_states (s s' s'' : CS.state) : Prop := *)
+  (* | mergeable_states_intro : forall t t' t'', *)
+  (*     mem_rel3 (CS.state_mem s, t) (CS.state_mem s', t') (CS.state_mem s'', t'') -> *)
+  (*     mergeable_states s s' s''. *)
 
   (* This "extensional" reading of compatible states depends directly on the
      partial programs concerned (implicitly through the section mechanism) and
      two runs synchronized by their traces. It is a rather strong notion, easy
      to work with and well suited to the purposes of the proof. *)
 
-(*
   Inductive mergeable_states (s s' s'' : CS.state) : Prop :=
     mergeable_states_intro : forall s0 s0' s0'' t t' t'' n n' n'',
       (* Well-formedness conditions. *)
@@ -315,6 +314,9 @@ Section Mergeable.
       Star sem   s0   t   s   ->
       Star sem'  s0'  t'  s'  ->
       Star sem'' s0'' t'' s'' ->
+      (* Sharing conditions.
+         NOTE: Think about possible redundancies. *)
+      mem_rel3 (CS.state_mem s, t) (CS.state_mem s', t') (CS.state_mem s'', t'') ->
       behavior_rel_behavior_all_cids n n'  (FTbc t) (FTbc t' ) ->
       behavior_rel_behavior_all_cids n n'' (FTbc t) (FTbc t'') ->
       mergeable_states s s' s''.
@@ -424,6 +426,7 @@ Section Mergeable.
   (*            eapply Hindstep with (t := [ev']); eauto. unfold E0. congruence. *)
   (* Qed. *)
 
+(*
   (* The following lemmas establish the connection between the mergeability
      relation and the application of the state merging functions. *)
   Lemma merge_mergeable_states_regs_program s s'' :
@@ -527,10 +530,15 @@ Section Mergeable.
     rewrite merge_mergeable_states_regs_context; try assumption.
     reflexivity.
   Qed.
+*)
+
+  (* Inversion pattern:
+inversion Hmerg as [s0 s0' s0'' t t' t'' n n' n'' Hwfp Hwfc Hwfp' Hwfc' Hmergeable_ifaces Hifacep Hifacec Hprog_is_closed Hprog_is_closed'' Hini Hini' Hini'' Hstar Hstar' Hstar'' Hmrel Htrel Htrel''].
+  *)
 
   (* Relations between mergeable states and program components. *)
-  Lemma mergeable_states_pc_same_component s s'' :
-    mergeable_states s s'' ->
+  Lemma mergeable_states_pc_same_component s s' s'' :
+    mergeable_states s s' s'' ->
     Pointer.component (CS.state_pc s) = Pointer.component (CS.state_pc s'').
   (* Proof. *)
   (*   intros Hmerg. *)
@@ -582,50 +590,53 @@ Section Mergeable.
   (*         Heveq: [_] = [_] |- _ => inversion Heveq; subst; reflexivity *)
   (*       end. *)
   (* Qed. *)
-  Admitted.
+  Admitted. (* RB: TODO: Should be fairly easy. *)
 
-  Lemma mergeable_states_program_to_program s s'' :
-    mergeable_states s s'' ->
+  Lemma mergeable_states_program_to_program s s' s'' :
+    mergeable_states s s' s'' ->
     CS.is_program_component s   ic ->
     CS.is_program_component s'' ic.
   Proof.
-    destruct s   as [[[[? ?] ?] pc  ] ?].
-    destruct s'' as [[[[? ?] ?] pc''] ?].
+    destruct s   as [[[? ?] ?] pc  ].
+    destruct s'' as [[[? ?] ?] pc''].
     unfold CS.is_program_component, CS.is_context_component, turn_of, CS.state_turn.
     intros Hmerge Hpc.
     pose proof mergeable_states_pc_same_component Hmerge as Hcomp. simpl in Hcomp.
     congruence.
   Qed.
 
-  Lemma mergeable_states_context_to_program s1 s2 :
-    mergeable_states s1 s2 ->
-    CS.is_context_component s1 ic ->
-    CS.is_program_component s2 ip.
+  Lemma mergeable_states_context_to_program s s' s'' :
+    mergeable_states s s' s'' ->
+    CS.is_context_component s ic ->
+    CS.is_program_component s'' ip.
   Proof.
     intros Hmerg.
     unfold CS.is_program_component, CS.is_context_component, turn_of, CS.state_turn.
-    destruct s1 as [[[[stack1 mem1] reg1] pc1] addrs1]; destruct s2 as [[[[stack2 mem2] reg2] pc2] addrs2].
+    destruct s as [[[stack1 mem1] reg1] pc1];
+      destruct s'' as [[[stack2 mem2] reg2] pc2].
     pose proof mergeable_states_pc_same_component Hmerg as Hpc; simpl in Hpc.
     rewrite <- Hpc; clear Hpc.
-    inversion Hmerg as [? ? ? ? _ _ _ _ _ _ [[_ Hdisj] _] _ _ _ _ Hini Hini'' Hstar Hstar'' _].
+    inversion Hmerg
+      as [? ? _ _ _ _ _ _ _ _ _ _ _ [[_ Hdisj] _] _ _ _ _ _ _ _ _ _ _ _ _ _].
     move: Hdisj.
     rewrite fdisjointC => /fdisjointP Hdisj.
     now auto.
   Qed.
 
-  Lemma mergeable_states_program_to_context s s'' :
-    mergeable_states s s'' ->
+  Lemma mergeable_states_program_to_context s s' s'' :
+    mergeable_states s s' s'' ->
     CS.is_program_component s ic ->
     CS.is_context_component s'' ip.
   Proof.
     intros Hmerg.
     unfold CS.is_program_component, CS.is_context_component, turn_of, CS.state_turn.
-    destruct s as [[[[stack mem] reg] pc] addrs]; destruct s'' as [[[[stack'' mem''] reg''] pc''] addrs''].
+    destruct s as [[[stack mem] reg] pc];
+      destruct s'' as [[[stack'' mem''] reg''] pc''].
     pose proof mergeable_states_pc_same_component Hmerg as Hpc; simpl in Hpc.
     rewrite <- Hpc.
-    inversion Hmerg as [s0 _ t _ _ _
+    inversion Hmerg as [s0 _ _ t _ _ _ _ _
                         Hwfp Hwfc _ _ Hmergeable_ifaces _ _ Hprog_is_closed _
-                        Hini _ Hstar _ _].
+                        Hini _ _ Hstar _ _ _ _ _].
     pose proof (CS.star_pc_domm_non_inform
                   _ _ Hwfp Hwfc Hmergeable_ifaces Hprog_is_closed Hini Hstar).
     intros Hn; destruct H.
@@ -635,15 +646,15 @@ Section Mergeable.
 
   (* RB: NOTE: Try to phrase everything either as CS.is_XXX_component, or as
      \[not]in. This is the equivalent of the old [PS.domm_partition]. *)
-  Lemma mergeable_states_notin_to_in s s'' :
-    mergeable_states s s'' ->
+  Lemma mergeable_states_notin_to_in s s' s'' :
+    mergeable_states s s' s'' ->
     Pointer.component (CS.state_pc s) \notin domm ip ->
     Pointer.component (CS.state_pc s) \in domm ic.
   Proof.
     intros Hmerg Hpc_notin.
-    inversion Hmerg as [[[[? ?] ?] pc] ? ? ? _ _
+    inversion Hmerg as [[[[? ?] ?] ?] _ ? ? _ ? _ _ _
                         Hwfp Hwfc _ _ Hmergeable_ifaces _ _ Hprog_is_closed _
-                        Hini _ Hstar _ _].
+                        Hini _ _ Hstar _ _ _ _ _].
     CS.unfold_states.
     pose proof (CS.star_pc_domm_non_inform
                   _ _ Hwfp Hwfc Hmergeable_ifaces Hprog_is_closed Hini Hstar) as Hpc.
@@ -654,9 +665,9 @@ Section Mergeable.
 
   (* RB: NOTE: Consider if the core of the lemma could be moved to CS, as is the
      case of its simpler variant, is_program_component_pc_notin_domm. *)
-  Lemma is_program_component_pc_in_domm s s'' :
+  Lemma is_program_component_pc_in_domm s s' s'' :
     CS.is_program_component s ic ->
-    mergeable_states s s'' ->
+    mergeable_states s s' s'' ->
     Pointer.component (CS.state_pc s) \in domm ip.
   Proof.
     intros Hpc Hmerge.
@@ -664,16 +675,16 @@ Section Mergeable.
       apply mergeable_states_program_to_context in Hcc; try assumption.
     unfold CS.is_context_component, turn_of, CS.state_turn in Hcc.
     rewrite (mergeable_states_pc_same_component Hmerge).
-    now destruct s'' as [[[[? ?] ?] ?] ?].
+    now destruct s'' as [[[? ?] ?] ?].
   Qed.
 
-  Lemma mergeable_states_program_component_domm mem gps regs pc addrs s'' :
-    mergeable_states (mem, gps, regs, pc, addrs) s'' ->
-    CS.is_program_component (mem, gps, regs, pc, addrs) ic ->
+  Lemma mergeable_states_program_component_domm mem gps regs pc s' s'' :
+    mergeable_states (mem, gps, regs, pc) s' s'' ->
+    CS.is_program_component (mem, gps, regs, pc) ic ->
     Pointer.component pc \in domm ip.
   Proof.
     intros Hmerge Hcomp.
-    change pc with (CS.state_pc (mem, gps, regs, pc, addrs)).
+    change pc with (CS.state_pc (mem, gps, regs, pc)).
     eapply is_program_component_pc_in_domm; last eassumption; assumption.
   Qed.
 
@@ -690,10 +701,12 @@ Section Mergeable.
       mergeable_stack (frame :: gps) (frame'' :: gps'').
 
   Lemma mergeable_states_mergeable_stack
-        gps1   mem1   regs1   pc1   addrs1
-        gps1'' mem1'' regs1'' pc1'' addrs1'' :
-    mergeable_states (gps1  , mem1  , regs1  , pc1  , addrs1  )
-                     (gps1'', mem1'', regs1'', pc1'', addrs1'') ->
+        gps1   mem1   regs1   pc1
+        st1'
+        gps1'' mem1'' regs1'' pc1'' :
+    mergeable_states (gps1  , mem1  , regs1  , pc1  )
+                     st1'
+                     (gps1'', mem1'', regs1'', pc1'') ->
     mergeable_stack gps1 gps1''.
   (* Proof. *)
   (*   intros Hmerg. *)
@@ -850,13 +863,14 @@ Section Mergeable.
   (*     + admit. *)
   (*     + admit. *)
   (*     + admit. *)
-  Admitted. (* RB: TODO: Check, repair induction principle.  *)
+  Admitted. (* RB: TODO: Should not be provable. Repair induction principle? *)
 
   Lemma mergeable_states_cons_domm
-        frame1   gps1   mem1   regs1   pc1   addrs1
-        frame1'' gps1'' mem1'' regs1'' pc1'' addrs1'' :
-    mergeable_states (frame1   :: gps1  , mem1  , regs1  , pc1  , addrs1  )
-                     (frame1'' :: gps1'', mem1'', regs1'', pc1'', addrs1'') ->
+        frame1   gps1   mem1   regs1   pc1
+        st1'
+        frame1'' gps1'' mem1'' regs1'' pc1'' :
+    mergeable_states (frame1   :: gps1  , mem1  , regs1  , pc1  ) st1'
+                     (frame1'' :: gps1'', mem1'', regs1'', pc1'') ->
     Pointer.component frame1 = Pointer.component frame1''.
   Proof.
     intros Hmerge.
